@base <https://version.link/>.

@prefix rdf: <http://www.w3.org/1999/02/22-rdf-syntax-ns#>.
@prefix rdfs: <http://www.w3.org/2000/01/rdf-schema#>.

# Core Schema

<>
  rdfs:label "version.link schema".

<Identity> a rdfs:Class;
  rdfs:label "Identity";
  rdfs:comment "Represents the Identity (concept). Identities are part of the Identity Graph.".

<Version> a rdfs:Class;
  rdfs:label "Version";
  rdfs:comment "A certain state of the Identity. A change in the Identity leads to a new Version.".

<Deprecated> a rdfs:Class;
  rdfs:label "Deprecated";
  rdfs:comment "Added to the last Version and the corresponding Identity, if a ChangeEvent leads to the deprecation of the Identity."

<VersionedIdentitySet> a rdfs:Class;
  rdfs:label "Versioned Identity Set";
  rdfs:comment "Represents the class of all the different objects of the versioned hierarchy."

<identity> a rdfs:Property;
  rdfs:range <Identity>;
  rdfs:domain <Version>;
  rdfs:label "identity";
  rdfs:comment "Links a Version to the corresponding Identity.".

<identityIdentifier> a rdfs:Property;
  rdfs:range rdfs:Literal;
  rdfs:domain <Version>;
  rdfs:label "identity identifier";
  rdfs:comment "Connects a literal identifier (not the complete IRI) of the corresponding Identity to the Version.".

<version> a rdfs:Property;
  rdfs:range <Version>;
  rdfs:domain <Identity>;
  rdfs:label "version";
  rdfs:comment "Links an Identity to the Version its currently based on.".

<predecessor> a rdfs:Property;
  rdfs:range <Version>;
  rdfs:domain <Version>;
  rdfs:label "predecessor";
  rdfs:comment "Links a certain Version to its predecessor Version. Can be used multiple times in a Version if multiple predecessor Versions exist (e.g. Combination).".

<successor> a rdfs:Property;
  rdfs:range <Version>;
  rdfs:domain <Version>;
  rdfs:label "successor";
  rdfs:comment "Links a certain Version to its successor Version. Can be used multiple times in a Version if multiple successor Versions exist (e.g. Separation).".

<startEvent> a rdfs:Property;
  rdfs:range <ChangeEvent>;
  rdfs:domain <Version>;
  rdfs:label "start event";
  rdfs:comment "Links a certain Version to the ChangeEvent that started the Version.".

<endEvent> a rdfs:Property;
  rdfs:range <ChangeEvent>;
  rdfs:domain <Version>;
  rdfs:label "end event";
  rdfs:comment "Links a certain Version to the ChangeEvent that ended the Version.". 

<inVersionedIdentitySet> a rdfs:Property;
  rdfs:range <ChangeEvent>;
  rdfs:domain <Version>;
  rdfs:domain <Identity>;
  rdfs:domain <VersionedIdentitySet>;
  rdfs:label "in versioned identity set";
  rdfs:comment "Connects an Identity, Version or ChangeEvent to a specific VersionedIdentitySet". 

<ChangeEvent> a rdfs:Class;
  rdfs:label "Change Event";
  rdfs:comment "A ChangeEvent connects different predecessors and successors of a specific change and has a single change type added. It is also possible to add multiple ChangeEvents with other change types and ChangeEvent that connect only a subset of all the predecessors and successors with more domain specific change types. The ChangeEvent should also have a date. ChangeEvents are instantaneous events with no duration.".

<InitialRecording> a rdfs:Class;
  rdfs:subClassOf <ChangeEvent>;
  rdfs:label "Initial Recording";
  rdfs:comment "Change type of a ChangeEvent. To create a Version without any predecessors.".

<ChangeOfName> a rdfs:Class;
  rdfs:subClassOf <ChangeEvent>;
  rdfs:label "Change Of Name";
  rdfs:comment "Change type of a ChangeEvent that corresponds to a change of name of the corresponding Identity".

<Separation> a rdfs:Class;
  rdfs:subClassOf <ChangeEvent>;
  rdfs:label "Separation";
  rdfs:comment "Change type of a ChangeEvent that corresponds to a separation of the corresponding Identity into multiple identities".

<Combination> a rdfs:Class;
  rdfs:subClassOf <ChangeEvent>;
  rdfs:label "Combination";
  rdfs:comment "Change type of a ChangeEvent that corresponds to a combination of the corresponding Identities into a single Identity".

<ChangeInHierarchy> a rdfs:Class;
  rdfs:subClassOf <ChangeEvent>;
  rdfs:label "Change In Hierarchy";
  rdfs:comment "Change type of a ChangeEvent that corresponds to a change of the position of the corresponding Identity in hierarchy (on the same level)".

<ChangeOfHierarchyLevel> a rdfs:Class;
  rdfs:subClassOf <ChangeEvent>;
  rdfs:label "Change In Hierarchy";
  rdfs:comment "Change type of a ChangeEvent that corresponds to a change of the hierarchy level of the corresponding Identity".